Fix some problems due to dep typed sep logic

src/MemMatch.v
@@ -114,7 +114,8 @@ Section MEMMATCH.
 
   Variable AEQ1 : DecEq AT1.
   Variable AEQ2 : DecEq AT2.
-  Variable V : Type.
+  Variable VT : Type.
+  Definition V {AT} := @const Type AT VT.
   Variable m1 : @mem AT1 AEQ1 V.
   Variable m2 : @mem AT2 AEQ2 V.
 
@@ -130,7 +131,7 @@ Section MEMMATCH.
   Variable AP1_ok : forall a1, indomain a1 m1 -> AP1 a1.
   Variable AP2_ok : forall a2, indomain a2 m2 -> AP2 a2.
 
-  Definition mem_atrans AT1 AEQ1 V AT2 AEQ2
+  Definition mem_atrans
     f (m : @mem AT1 AEQ1 V) (m' : @mem AT2 AEQ2 V) (P : AT1 -> Prop) :=
     forall a, P a -> m a = m' (f a).
 
@@ -206,6 +207,7 @@ Section MEMMATCH.
       apply mem_ainv_any; auto.
       replace (atrans (ainv a)) with a; auto.
       apply eq_sym; apply HInv; auto.
+      apply H; auto.
       apply HInv; auto.
 
       destruct (indomain_dec a m2); auto.
@@ -231,12 +233,16 @@ Section MEMMATCH.
     Lemma mem_ainv_mem_upd : forall a v (ap : AP2 a),
       mem_atrans atrans (Mem.upd m1 (ainv a) v) (Mem.upd m2 a v) AP1.
     Proof.
-      intros; unfold mem_atrans, Mem.upd; intro x.
-      destruct (AEQ1 x (ainv a)); destruct (AEQ2 (atrans x) a); auto.
+      intros; unfold mem_atrans; intro x.
+      destruct (AEQ1 x (ainv a)); destruct (AEQ2 (atrans x) a); simpl_upd; auto.
+      rewrite e0; simpl_upd.
+      rewrite <- e; simpl_upd.
+      auto.
+
       contradict n; subst.
       apply HInv; auto.
 
-      intros; subst.
+      intros.
       contradict n.
       erewrite cond_inv_rewrite_left; eauto.
     Qed.
